tests/reference/__init__.py
@@ -1,0 +1,1 @@
+"""Pure reference models used by differential tests."""
